Fix encoding of functions that use nat and more rewrite of Primitives.thy

Cook_Levin_IMP/IMP-_To_SAS+/IMP--_To_SAS++/IMP_Minus_Minus_To_SAS_Plus_Plus_State_Translations.thy
@@ -2,12 +2,12 @@
 
 section "IMP-- to SAS++ State Translations"
 
-theory IMP_Minus_Minus_To_SAS_Plus_Plus_State_Translations 
+theory IMP_Minus_Minus_To_SAS_Plus_Plus_State_Translations
   imports SAS_Plus_Plus IMP_Minus_Minus_Small_StepT
 begin
 
 text \<open> We define a translation between IMP-- states and SAS++ states. For this purpose, it is useful
-      to think of IMP-- states as not only a map from registers to bits, but rather a pair of a 
+      to think of IMP-- states as not only a map from registers to bits, but rather a pair of a
       computation and such a map. The translated SAS++ states is a map assigning the computation
       to the special variable PC, and otherwise mapping register names to the bit values they
       had in the original IMP-- state. \<close>
@@ -20,42 +20,42 @@ type_synonym sas_state = "(variable, domain_element) State_Variable_Representati
 type_synonym imp_state = state
 
 definition imp_minus_state_to_sas_plus :: "(com \<times> imp_state) \<Rightarrow> sas_state" where
-"imp_minus_state_to_sas_plus ci = ((\<lambda>x. Some (EV x)) \<circ>\<^sub>m (snd ci)
+  "imp_minus_state_to_sas_plus ci = ((\<lambda>x. Some (EV x)) \<circ>\<^sub>m (snd ci)
   \<circ>\<^sub>m (\<lambda>x. (case x of VN v \<Rightarrow> Some v)))
   (PC \<mapsto> PCV (fst ci))"
 
 
 definition sas_plus_state_to_imp_minus:: "sas_state \<Rightarrow> (com \<times> imp_state)" where
-"sas_plus_state_to_imp_minus ss = ((case (the (ss PC)) of (PCV c) \<Rightarrow> c), 
+  "sas_plus_state_to_imp_minus ss = ((case (the (ss PC)) of (PCV c) \<Rightarrow> c),
   (\<lambda>x. (case x of EV y \<Rightarrow> Some y | _ \<Rightarrow> None)) \<circ>\<^sub>m ss \<circ>\<^sub>m (\<lambda>x. Some (VN x)))"
 
 definition sane_sas_plus_state:: "sas_state \<Rightarrow> bool" where
-"sane_sas_plus_state ss \<equiv> (\<exists>x. ss PC = Some (PCV x)) \<and> 
+  "sane_sas_plus_state ss \<equiv> (\<exists>x. ss PC = Some (PCV x)) \<and>
   (\<forall>v. VN v \<in> dom ss \<longrightarrow> (\<exists>x. ss (VN v) = Some (EV x)))"
 
 lemma sas_plus_state_to_imp_minus_imp_minus_state_to_sas_plus[simp]:
-  "sas_plus_state_to_imp_minus (imp_minus_state_to_sas_plus (c, is)) = (c, is)" 
+  "sas_plus_state_to_imp_minus (imp_minus_state_to_sas_plus (c, is)) = (c, is)"
 proof -
   have "(snd (sas_plus_state_to_imp_minus (imp_minus_state_to_sas_plus (c, is)))) x = is x" for x
-    by (auto simp: imp_minus_state_to_sas_plus_def sas_plus_state_to_imp_minus_def 
+    by (auto simp: imp_minus_state_to_sas_plus_def sas_plus_state_to_imp_minus_def
         map_comp_def option.case_eq_if)
   then show ?thesis
     by (auto simp: imp_minus_state_to_sas_plus_def sas_plus_state_to_imp_minus_def)
 qed
 
-lemma imp_minus_state_to_sas_plus_sas_plus_state_to_imp_minus[simp]: 
+lemma imp_minus_state_to_sas_plus_sas_plus_state_to_imp_minus[simp]:
   assumes "sane_sas_plus_state ss "
-  shows "imp_minus_state_to_sas_plus (sas_plus_state_to_imp_minus ss) = ss" 
+  shows "imp_minus_state_to_sas_plus (sas_plus_state_to_imp_minus ss) = ss"
 proof -
   have "(imp_minus_state_to_sas_plus (sas_plus_state_to_imp_minus ss)) x = ss x" for x using assms
-    by (fastforce simp: imp_minus_state_to_sas_plus_def sas_plus_state_to_imp_minus_def 
+    by (fastforce simp: imp_minus_state_to_sas_plus_def sas_plus_state_to_imp_minus_def
         sane_sas_plus_state_def option.case_eq_if map_comp_def split: variable.splits)
   then show ?thesis by (auto simp: imp_minus_state_to_sas_plus_def sas_plus_state_to_imp_minus_def)
 qed
 
-lemma imp_minus_state_to_sas_plus_of_same_c_eq_iff[simp]: 
+lemma imp_minus_state_to_sas_plus_of_same_c_eq_iff[simp]:
   "(imp_minus_state_to_sas_plus (c, s1) = imp_minus_state_to_sas_plus (c, s2))
-  \<longleftrightarrow> s1 = s2" 
+  \<longleftrightarrow> s1 = s2"
 proof
   assume a: "imp_minus_state_to_sas_plus (c, s1) = imp_minus_state_to_sas_plus (c, s2)"
   have "\<forall>v. (s1 v = s2 v)"
@@ -69,53 +69,114 @@ proof
   then show "s1 = s2" by auto
 qed auto
 
-lemma snd_sas_plus_state_to_imp_minus_updated[simp]: 
+lemma snd_sas_plus_state_to_imp_minus_updated[simp]:
   "snd (sas_plus_state_to_imp_minus
-                (imp_minus_state_to_sas_plus (c, is)(VN x \<mapsto> y))) 
+                (imp_minus_state_to_sas_plus (c, is)(VN x \<mapsto> y)))
     = is(x := (case y of EV y' \<Rightarrow> Some y' | _ \<Rightarrow> None))"
-  by (auto simp: imp_minus_state_to_sas_plus_def sas_plus_state_to_imp_minus_def 
-       Let_def map_comp_def option.case_eq_if)
+  by (auto simp: imp_minus_state_to_sas_plus_def sas_plus_state_to_imp_minus_def
+      Let_def map_comp_def option.case_eq_if)
 
-lemma imp_minus_state_to_sas_plus_PC[simp]: 
-  "(imp_minus_state_to_sas_plus (c1, is)) PC = Some (PCV c1)" 
+lemma imp_minus_state_to_sas_plus_PC[simp]:
+  "(imp_minus_state_to_sas_plus (c1, is)) PC = Some (PCV c1)"
   by (simp add: imp_minus_state_to_sas_plus_def)
 
-lemma imp_minus_state_to_sas_plus_VN_Some_iff[simp]: 
-  "(imp_minus_state_to_sas_plus (c, is) (VN x) = Some (EV y)) 
+lemma imp_minus_state_to_sas_plus_VN_Some_iff[simp]:
+  "(imp_minus_state_to_sas_plus (c, is) (VN x) = Some (EV y))
   \<longleftrightarrow> (is x = Some y)"
   by(auto simp: imp_minus_state_to_sas_plus_def map_comp_Some_iff)
 
-lemma imp_minus_state_to_sas_plus_eq_Some_non_zero_iff[simp]: 
+lemma imp_minus_state_to_sas_plus_eq_Some_non_zero_iff[simp]:
   "imp_minus_state_to_sas_plus (c, is) (VN x) = Some y \<Longrightarrow>
        (y \<noteq> EV (Num 0)) \<longleftrightarrow> (is x \<noteq> Some (Num 0))"
   by(auto simp: imp_minus_state_to_sas_plus_def map_comp_Some_iff)
 
-lemma imp_minus_state_to_sas_plus_map_le_then: "imp_minus_state_to_sas_plus (c, I) \<subseteq>\<^sub>m I' 
+lemma imp_minus_state_to_sas_plus_map_le_then: "imp_minus_state_to_sas_plus (c, I) \<subseteq>\<^sub>m I'
   \<Longrightarrow> I \<subseteq>\<^sub>m snd (sas_plus_state_to_imp_minus I')"
   apply(auto simp: imp_minus_state_to_sas_plus_def sas_plus_state_to_imp_minus_def)
-   apply(simp add: map_le_def map_comp_def)
-   apply(auto split: option.splits domain_element.splits)
-     apply (metis domIff option.distinct option.simps variable.simps)
-   apply (metis domI domain_element.inject option.inject option.simps variable.distinct variable.simps)
-  by (metis (mono_tags, lifting) domI domain_element.distinct option.inject option.simps 
+  apply(simp add: map_le_def map_comp_def)
+  apply(auto split: option.splits domain_element.splits)
+  apply (metis domIff option.distinct option.simps variable.simps)
+  apply (metis domI domain_element.inject option.inject option.simps variable.distinct variable.simps)
+  by (metis (mono_tags, lifting) domI domain_element.distinct option.inject option.simps
       variable.distinct variable.simps)
 
 
-lemma map_of_map_VN_EV: "map_of (map (\<lambda>v. (VN v, EV y)) vs) (VN a) = 
+lemma map_of_map_VN_EV: "map_of (map (\<lambda>v. (VN v, EV y)) vs) (VN a) =
   map_option EV (map_of (map (\<lambda>v. (v, y)) vs) a)"
   apply(induction vs) by auto
 
-lemma map_leq_imp_minus_state_to_sas_plus_iff: 
+lemma map_leq_imp_minus_state_to_sas_plus_iff:
   "map_of (map (\<lambda>v. (VN v, EV y)) vs)(PC \<mapsto> PCV c) \<subseteq>\<^sub>m imp_minus_state_to_sas_plus (c, is)
   \<longleftrightarrow> map_of (map (\<lambda>v. (v, y)) vs) \<subseteq>\<^sub>m is"
-  by(auto simp: imp_minus_state_to_sas_plus_def map_le_def map_comp_def map_of_SomeD 
+  by(auto simp: imp_minus_state_to_sas_plus_def map_le_def map_comp_def map_of_SomeD
       dom_map_of_conv_image_fst map_of_map_VN_EV split: option.splits)
 
-lemma dom_snd_sas_plus_state_to_imp_minus:  "sane_sas_plus_state ss 
-  \<Longrightarrow> dom (snd (sas_plus_state_to_imp_minus ss)) 
-  = { v |v. VN v \<in> dom ss }" 
-  by(fastforce simp: sane_sas_plus_state_def sas_plus_state_to_imp_minus_def map_comp_Some_iff 
+lemma dom_snd_sas_plus_state_to_imp_minus:  "sane_sas_plus_state ss
+  \<Longrightarrow> dom (snd (sas_plus_state_to_imp_minus ss))
+  = { v |v. VN v \<in> dom ss }"
+  by(fastforce simp: sane_sas_plus_state_def sas_plus_state_to_imp_minus_def map_comp_Some_iff
       split: option.splits)
-  
+
+instantiation domain_element :: order_bot
+begin
+
+fun less_eq_domain_element :: "domain_element \<Rightarrow> domain_element \<Rightarrow> bool" where
+  "less_eq_domain_element (EV b1) (EV b2) \<longleftrightarrow> b1 \<le> b2"
+| "less_eq_domain_element (PCV c1) (PCV c2) \<longleftrightarrow> c1 \<le> c2"
+| "less_eq_domain_element (EV _) _ \<longleftrightarrow> True"
+| "less_eq_domain_element _ (EV _) \<longleftrightarrow> False"
+
+definition less_domain_element :: "domain_element \<Rightarrow> domain_element \<Rightarrow> bool" where
+  "less_domain_element c1 c2 = (c1 \<le> c2 \<and> \<not> c2 \<le> c1)"
+
+definition bot_domain_element :: "domain_element" where
+  "bot_domain_element = EV bot"
+
+instance
+proof(standard, goal_cases)
+  case 1 show ?case by (simp add: less_domain_element_def)
+next
+  case 2 show ?case
+    using less_eq_domain_element.elims(3) by fastforce
+next
+  case 3 thus ?case by (fastforce elim: less_eq_domain_element.elims)
+next
+  case 4 thus ?case by (fastforce elim: less_eq_domain_element.elims)
+next
+  case 5 show ?case unfolding bot_domain_element_def using less_eq_domain_element.elims
+    by (metis IMP_Minus_Minus_To_SAS_Plus_Plus_State_Translations.domain_element.exhaust bot_bit_def
+        less_eq_bit.simps(1) less_eq_domain_element.simps(1) less_eq_domain_element.simps(3))
+qed
+end
+
+instantiation variable :: order_bot
+begin
+
+fun less_eq_variable :: "variable \<Rightarrow> variable \<Rightarrow> bool" where
+  "less_eq_variable (VN v1) (VN v2) \<longleftrightarrow> v1 \<le> v2"
+| "less_eq_variable PC _ \<longleftrightarrow> True"
+| "less_eq_variable _ PC \<longleftrightarrow> False"
+
+definition less_variable :: "variable \<Rightarrow> variable \<Rightarrow> bool" where
+  "less_variable c1 c2 = (c1 \<le> c2 \<and> \<not> c2 \<le> c1)"
+
+definition bot_variable :: "variable" where
+  "bot_variable = PC"
+
+instance
+proof(standard, goal_cases)
+  case 1 show ?case by (simp add: less_variable_def)
+next
+  case 2 show ?case
+    using less_eq_variable.elims(3) by fastforce
+next
+  case 3 thus ?case by (fastforce elim: less_eq_variable.elims)
+next
+  case 4 thus ?case by (fastforce elim: less_eq_variable.elims)
+next
+  case 5 show ?case unfolding bot_variable_def by simp
+qed
+end
+
 
 end
